compilation/MainCompileScript.sml
@@ -1,8 +1,0 @@
-open preamble compilationLib MainProgTheory
-
-val _ = new_theory"MainCompile";
-
-val main_compiled = save_thm("main_compiled",
-  compile_x64 1000 1000 "check_count" main_prog_def);
-
-val _ = export_theory();
