compilation/proofs/check_countProofScript.sml
@@ -1,12 +1,12 @@
 open preamble
      semanticsPropsTheory backendProofTheory x64_configProofTheory
-     MainProgTheory MainCompileTheory
+     check_countProgTheory check_countCompileTheory
 
 val _ = new_theory"check_countProof";
 
 val check_count_io_events_def = new_specification("check_count_io_events_def",
   ["check_count_io_events","check_count_fs"],
-  main_correct |> Q.GENL[`init_out`,`cls`,`fs`] |> Q.SPEC`""`
+  check_count_correct |> Q.GENL[`init_out`,`cls`,`fs`] |> Q.SPEC`""`
   |> SIMP_RULE bool_ss [SKOLEM_THM,GSYM RIGHT_EXISTS_IMP_THM,RIGHT_EXISTS_AND_THM,APPEND]);
 
 val (check_count_sem,check_count_output) = check_count_io_events_def |> SPEC_ALL |> UNDISCH |> CONJ_PAIR
@@ -14,7 +14,7 @@ val (check_count_not_fail,check_count_sem_sing) =
   MATCH_MP semantics_prog_Terminate_not_Fail check_count_sem |> CONJ_PAIR
 
 val compile_correct_applied =
-  MATCH_MP compile_correct main_compiled
+  MATCH_MP compile_correct check_count_compiled
   |> SIMP_RULE(srw_ss())[LET_THM,ml_progTheory.init_state_env_thm,GSYM AND_IMP_INTRO]
   |> C MATCH_MP check_count_not_fail
   |> C MATCH_MP x64_backend_config_ok
